Enumeration of normal form

theories/inttrie.v
@@ -421,5 +421,143 @@ Qed.
 
 Definition pres_triesize := foldl max 0 (pgen P) + 1.
 
+Lemma pgen_triesize :
+  all (<%O^~ max_length) (pgen P) -> correctrelat (prelat P) (<%O^~ pres_triesize).
+Proof.
+rewrite /pres_triesize => H; apply: pgen_size; move: H.
+have : (0 < max_length)%O by [].
+elim: (pgen P) (0) => // [g0 g IHg] /= i lti.
+case/andP => ltg0 alllt; apply/andP; split; first last.
+  by apply: IHg => //; rewrite ltintE maxintE gtn_max -!ltintE lti ltg0.
+elim: g alllt {IHg} i lti g0 ltg0 => [| g1 g IHg] /=.
+  move=> _ i lti g ltg; rewrite ltintE to_natD to_nat1 addn1 maxintE.
+    by rewrite ltnS leq_maxr.
+  apply: (leq_trans (n := (to_nat max_length).+1)).
+    by rewrite ltnS gtn_max -!ltintE lti ltg.
+  by apply/ltP; rewrite -Z2Nat.inj_lt.
+case/andP => [ltg1 alllt] i lti g0 ltg0.
+have -> : max (max i g0) g1 = max (max i g1) g0.
+  apply: int_to_nat_inj.
+  rewrite [LHS]maxintE [in LHS]maxintE [RHS]maxintE [in RHS]maxintE.
+  by rewrite -!maxnA [maxn (to_nat g1) _]maxnC.
+apply: IHg => //=.
+by rewrite ltintE maxintE gtn_max -!ltintE lti ltg1.
+Qed.
+
 End Size.
 
+
+Section EnumNormalForms.
+
+Variable (P: pres int) (trielen : int).
+Hypothesis convP : convergent (prelat P).
+Hypothesis trielenOk : (trielen <= max_length)%O.
+Hypothesis genPlen : all (<%O^~ trielen) (pgen P).
+
+Implicit Types (u v w : word int) (norf : seq (word int)).
+
+Let corrlen :=  pgen_size genPlen.
+Let Ptrie := mktrie trielen (prelat P).
+
+Definition normal_sz (n : nat) u :=
+  [&& size u == n, u \in words_of P & normal (prelat P) u].
+Definition enum_normal_next norf :=
+  [seq x <- [seq g :: w | g <- pgen P, w <- norf] |
+    ~~ trie_rewrites1_front Ptrie x].
+Definition enum_normal n := iter n enum_normal_next [:: [::]].
+
+Lemma normal_sz0 : normal_sz 0 [::].
+Proof. by rewrite /normal_sz /=; apply normal0; case: convP. Qed.
+
+Lemma normal_sz_enum_normal n : all (normal_sz n) (enum_normal n).
+Proof.
+elim: n => [| n]; first by rewrite /= normal_sz0.
+rewrite {2}/enum_normal /= -/(enum_normal n).
+move: (enum_normal n) => norf /allP /= allnorf; apply/allP => /= [[| u0 u]].
+  by rewrite mem_filter => /andP[_ /allpairsP[[/= u0 u []]]].
+rewrite mem_filter => /andP[nrew].
+case/allpairsP => /= - [v0 v]/= [ugen unor []] equ0 equ; subst v0 v.
+have := allnorf u unor; rewrite /normal /= /normal_sz /= eqSS.
+case: eqP => //= _.
+have -> : (u0 :: u \in words_of P) = (u \in words_of P).
+  by rewrite !unfold_in /words_of /= ugen.
+case: (u \in _) => //=.
+rewrite /normal /= cat_eq0 map_eq0 => /eqP ->.
+rewrite eqxx andbT.
+have -> // := (trie_rewrites1_front0 trielenOk corrlen).
+by case: trie_rewrites1_front nrew.
+Qed.
+
+Lemma count_mem_enum_normal n u :
+  normal_sz n u -> count_mem u (enum_normal n) = 1%N.
+Proof.
+elim: n u => [|n]; first by case.
+rewrite {2}/enum_normal /= -/(enum_normal n).
+move: (enum_normal n) => norf Hn [|u0 u] //=.
+rewrite /normal_sz /= eqSS.
+have -> : (u0 :: u \in words_of P) = (u0 \in pgen P) && (u \in words_of P).
+  by rewrite !unfold_in /words_of /=.
+case: (boolP (u0 \in pgen P)) => [u0P |]; rewrite ?andbF ?andbT //=.
+rewrite /normal /= cat_eq0 map_eq0 -/(normal _ u) [X in [&& _, _ & X]]andbC.
+rewrite !andbA andbC -!andbA -/(normal_sz n u) andbC.
+case/andP => {}/Hn unorf /eqP rew0.
+rewrite count_filter /normal /= count_flatten sumnE 2!big_map.
+rewrite (bigD1_seq _ u0P (uniq_pgen P)) /= big1_seq ?addn0; first last.
+  move=> /= i /andP[/negbTE neq _].
+  rewrite -count_filter; apply/count_memPn/negP.
+  rewrite mem_filter => /andP[_ /mapP[/= x _ /eqP]].
+  by rewrite eqseq_cons eq_sym neq.
+rewrite count_map -[RHS]unorf; apply eq_count => /= v /=.
+rewrite eqseq_cons eqxx /=; case: eqP => //= {v}->.
+case: trie_rewrites1_frontP => //= w.
+by rewrite rew0.
+Qed.
+
+Lemma uniq_enum_normal n : uniq (enum_normal n).
+Proof.
+have /allP /= allnorf := normal_sz_enum_normal n.
+apply: count_mem_uniq => /= u.
+case: (boolP (u \in _)) => [/allnorf/count_mem_enum_normal -> // | /= unotin].
+exact/count_memPn.
+Qed.
+
+Lemma mem_enum_normalP n u : (u \in enum_normal n) = normal_sz n u.
+Proof.
+have /allP /= allnorf := normal_sz_enum_normal n.
+case: (boolP (u \in _)) => [/allnorf -> // | /= unotin].
+apply/esym; apply/contraNF: unotin => /count_mem_enum_normal.
+by rewrite -has_pred1 has_count => ->.
+Qed.
+
+End EnumNormalForms.
+
+
+Require Import rewcert wfsizelexi.
+
+Module Example.
+
+Definition P := make_pres [::0; 1]
+  [::
+   ([::1;0], [::0;1]);
+   ([::0;0;0], [::0;1]);
+   ([::1;1], [::1])
+  ].
+
+Theorem final_ok : convergent (prelat P).
+Proof.
+apply: diamond.
+  apply (decreasing_wf (@lt_sizelexi_stable _ int) sizelexi_int_wf).
+  by native_cast_no_check is_true_true.
+pose trielen := pres_triesize P.
+have lenOk : (trielen <= PArray.max_length)%O by [].
+have relOk : correctrelat (prelat P) (<%O^~ trielen)
+  by apply: pgen_size.
+apply (spair_confluence_loopP (trie_rewrites1P lenOk relOk) (fuel := 10)).
+rewrite spair_confluence_loop_trieE.
+by native_cast_no_check is_true_true.
+Qed.
+
+Eval compute in flatten (traject (enum_normal_next P 2) [:: [::]] 4).
+Eval compute in (iter 4 (enum_normal_next P 2) [:: [::]]).
+
+End Example.
