theories/samples/rennertypeD51.v
@@ -22472,5 +22472,22 @@ Definition cert : pres_cert := [:: add_rel [::11;7] [::11]
 
 Definition final_order := [::0;1;2;3;4;5;6;7;8;9;10;11].
 
-
 Load "footer_trie.v".
+
+
+(* 
+From mathcomp Require Import ssrnat path.
+(* final_ok
+     : convergent (prelat present_final) *)
+
+Eval native_compute in
+  foldl (fun acc s => acc + of_nat (seq.size s)) 0
+    (traject (enum_norf_next present_final 12) [:: [::]] 40).
+
+Eval native_compute in
+  map (fun s => of_nat (seq.size s))
+    (traject (enum_norf_next present_final 12) [:: [::]] 36).
+
+Eval native_compute in
+  foldl maxn 0%N [seq seq.size r.1 | r <- prelat present_final].
+*)
